examples/rel/Equivalence.fst
@@ -12,12 +12,11 @@ let if_left a e e1 e2 h0 = ()
 
 (* then trying to go for non-trivial pre- and postconditions *)
 let if_left_wp (a:Type)
-    (epre:_)  (epost:_)  (e:(unit -> ST bool epre epost))
-    (e1pre:_) (e1post:_) (e1:(unit -> ST a e1pre e1post))
-    (e2pre:_) (e2post:_) (e2:(unit -> ST a e2pre e2post)) (h0:heap) :
-  Lemma (requires (epre h0 /\ reify (e()) h0 == (true, h0)))
-        (ensures ((epre h0 /\ e1pre h0 /\ e2pre h0) ==>
-                     reify (if e() then e1()
-                                   else e2()) h0 == reify (e1()) h0))
-  = ()
-(* Stuck: assertion fail for the e1() and e2(), still no clue why *)
+    (epre:_)  (epost:_) (e1pre:_) (e1post:_) (e2pre:_) (e2post:_) 
+    (e:(unit -> ST bool epre epost))
+    (e1:(unit -> ST a e1pre e1post))
+    (e2:(unit -> ST a e2pre e2post)) (h0:heap{epre h0 /\ e1pre h0 /\ e2pre h0 /\
+                                             reify (e()) h0 == (true, h0)}) :
+  Lemma (reify (if refine_st e () then e1 () else e2 ()) h0 ==  //using refine_st to establish that after e () the heap remains same
+         reify (e1 ()) h0)
+  = ignore (reify (refine_st e ()) h0) (* AR: not sure why this is required *)
